% !TeX root = ../SigSysBoxen.tex

\begin{abox}
	\mathcal{Z}\{x[-k]\} = \sum_{k = -\infty}^{\infty}x[-k]z^{-k} \underset{(k = -k')}{\overset{k' = -k}{=}} \sum_{k' = -\infty}^{\infty}x[k']z^{k'} = \sum_{k' = -\infty}^{\infty}x[k'] \cdot \left(\frac{1}{z}\right)^{-k'} = X\left(\frac{1}{z}\right)
\end{abox}

\begin{abox}
	x[0] = \lim\limits_{z \rightarrow \infty} X(z)
\end{abox}

\begin{abox}
	\lim\limits_{k\rightarrow\infty}x[k] = \lim\limits_{z\rightarrow 1}(z - 1) \cdot X(z)
\end{abox}

\begin{abox}
	\mathcal{Z}\{\alpha^{k-1} \cdot \epsilon[k-1]\} = z^{-1} \cdot \mathcal{Z}\{\alpha^k \cdot \epsilon[k]\} = z^{-1} \cdot \frac{z}{z - \alpha} = \frac{1}{z - \alpha}
\end{abox}

\begin{abox}
	\mathcal{Z}\{A \cdot\alpha^{k-k_0} \cdot\epsilon[k - k_0]\} = A \cdot z^{-k} \cdot \mathcal{Z}\{\alpha^k\epsilon[k]\} = A \cdot z^{-k_0} \cdot \frac{z}{z - \alpha} = \frac{A \cdot z^{-(k_0-1)}}{z - \alpha}
\end{abox}

\begin{abox}
	\mathcal{Z}\{k\cdot\alpha^k\cdot\epsilon[k]\} &= -z \cdot \frac{d}{dz}\mathcal{Z}\{\alpha^k\epsilon[k]\} = -z \cdot \left(\frac{z}{z - \alpha}\right)' \\
	&= -z \cdot \left(\frac{1 \cdot (z - \alpha) - z \cdot 1}{(z - \alpha)^2}\right) = \frac{\alpha\cdot z}{(z - \alpha)^2}
\end{abox}

\begin{abox}
	Y(z) = H(z) \cdot X(z)
\end{abox}

\begin{abox}
	H(z) = \frac{Y(z)}{X(z)}
\end{abox}

\begin{abox}
	h[k] &= (1 + p)^k \cdot \epsilon[k]\\
	H(z) &= \frac{z}{z - (1 + p)}
\end{abox}

\begin{abox}
	y[k + 1] &= y[k] \cdot (1 + p) +  x[k + 1]\\
	&\ztrans\\
	Y(z) &= Y(z) \cdot (1 + p) + zX(z) \Leftrightarrow Y(z)(z - (1 + p)) = zX(z)
\end{abox}
%111
\begin{abox}
	H(z) := \frac{Y(z)}{X(z)} = \frac{z}{z - (1 + p)}
\end{abox}






\begin{abox}
	x[k] &= x_0 \cdot \epsilon[k]\\
	&\ztrans\\
	X(z) &= x_0 \cdot \frac{z}{z-1}
\end{abox}

\begin{abox}
	Y(z)= H(z) \cdot X(z) = \frac{z}{z-(a+p)}\cdot x_0 \cdot \frac{z}{z-q} = x_0 \cdot z^2 \cdot \frac{1}{\left(z-\left(a+p\right)\right)\cdot\left(z-1\right)}
\end{abox}

\begin{abox}
	\frac{1}{\left(z-\left(a+p\right)\right)\cdot\left(z-1\right)} &= \frac{p^{-1}}{z-(a+p)} - \frac{p^{-1}}{z-1}\\
\end{abox}

\begin{abox}
	\frac{p^{-1}}{z-(a+p)} \Laplace p^{-1}(a+p)^{K-1} \epsilon[K-1]
	\text{ und }\\
	\frac{p^{-1}}{z-1} \Laplace p^{-1}1^{K-1}\epsilon[K-1] = p^{-1}\epsilon[K-1]
\end{abox}

\setcounter{BoxCounter}{116}
% 117
\begin{abox}
	\sum_{i=0}^{n}\alpha_i y[k-i] &= \sum_{i=N-M}^{N}\beta_i x[k-i] &(a_0 \ne 0, \beta_{N-M} \ne 0)\\
	&\ztrans\\
	\sum_{i=0}^{N}\alpha_i\cdot z^{-i} \cdot Y(z) &= \sum_{i= N-M}^{N} \beta_i \cdot z^{-i} \cdot X(z)\\
	\Leftrightarrow  Y(z) \cdot \sum_{i=0}^{N}\alpha_i\cdot z^{-i} &= X(z) \cdot \sum_{i= N-M}^{N} \beta_i \cdot z^{-i}
\end{abox}

\begin{abox}
	H(z):= \frac{Y(z)}{X(z)} &=\frac{\sum_{i= N-M}^{N} \beta_i \cdot z^{-i}}{\sum_{i=0}^{N}\alpha_i\cdot z^{-i}}\\
	&=\frac{\sum_{i= N-M}^{N} \beta_i \cdot z^{N-i}}{\sum_{i=0}^{N}\alpha_i\cdot z^{N-i}}\\
	&= \frac{\beta_{N-M}\cdot z^M + \beta_{N-M+1}\cdot z^{M-1} + ... + \beta_N}{\alpha_0 \cdot z^N + \alpha_1 \cdot z^{N-1} + ... + \alpha_N}
\end{abox}

\begin{abox}
	y(k) = \frac{1}{\alpha_0}\left(\sum_{i=N-M}^{N}\beta_ix[k-i] - \sum_{i=1}^{N}\alpha_iy[k-i]\right)
\end{abox}


\begin{abox}
	h[k] &= 3 \cdot (\frac15)^k \cdot epsilon[k] + 2 \cdot (\frac12)^k \cdot \epsilon[k]\\
	&\ztrans\\
	H(z) &= 3\cdot \frac{z}{z-\frac15} + 2 \cdot \frac{z}{z-\frac12} = \frac{15z}{5z-1} + \frac{4z}{2z-1}\\	
	&= \frac{15z(2z-1) + 4z(5z-1)}{(5z-1)(2z-1)} = \frac{50z^2 - 19z}{10z^2 - 7z +1}
\end{abox}

\begin{abox}
	\alpha_0 = a_2 = 10, \alpha_1 = -7, \alpha_1 = 1 \text{ und } \beta_0=50,\beta_1=-19,\beta_2=0
\end{abox}

\begin{abox}
	10y[k]-7y[k-1]+1y[k-2] = 50x[k]-19x[k-1] \text{ bzw. Ã¤quivalent }\\
	y[k]=\frac{1}{10}\cdot  \left(50x[k]-19x[k-1]+7y[k-1]-y[k-2]\right)
\end{abox}

\begin{abox}
	h[k] &= 3 \cdot 5^{-(k+2)}\epsilon[k+2] + 2 \cdot 2^{-k} \epsilon[k]\\
	&\ztrans\\
	H(z)&= 3 \cdot z^2 \frac{z}{z-\frac15} + 2 \cdot \frac{z}{z-\frac12}\\ &= \frac{15z^3}{5z-1}+\frac{4z}{2z-1} = \frac{30z^4 - 15z^3 + 20z^2 - 4z}{10z^2 - 7z + 1}\\ &(\Rightarrow M=4, N=2)
\end{abox}

\begin{abox}
	\alpha_0=a_{2-0}=10, \alpha_1 = -7, \alpha_2 = 1 \text{ und }\\
	\beta_{-2} = b_4 =30, \beta_{-1}= 15, \beta_0=20, \beta_1 = -4
\end{abox}

\begin{abox}
	10y[k] -7y[k-1] + y[k-2] = 30x[k+2]-15[k+1]+20x[k]-4x[k-1]\\
	y[k] =\frac{1}{10} \left(30x[k+2]-15[k+1]+20x[k]-4x[k-1]+7y[k-1] - y[k-2]\right)
\end{abox}

\begin{abox}
	y[k-2] = \frac{1}{10}\left(30x[k+2]-15[k-1]+20x[k-2]-4x[k-3]+7y[k-3] - y[k-4]\right)
\end{abox}

\begin{abox}
	x[k] = \mathcal{Z}^{-1}\left\lbrace X(z)\right\rbrace  = \mathcal{Z}^1\left\lbrace \sum_{k=-\infty}^{\infty}x[k]z^{-k}\right\rbrace
\end{abox}

\begin{abox}
	Y(z) = 1 \cdot z^{-1} - \frac12 z^{-2} + \frac13 z^{-3} - \frac14 z^{-4} + ... + \frac{(-1)^{k+1}}{k}z^{-k} + ...
\end{abox}

\begin{abox}
	y[k] = \begin{cases}
		0 &, k \leq 0\\ (-1)^{k+1}\cdot\frac1k &, k>0
	\end{cases}
\end{abox}

\begin{abox}
	Y(z) \overset{!}{=} \frac{A_1}{z-\lambda_1} + \frac{A_2}{z-\lambda_2} + ... + \frac{A_n}{z-\lambda_n}
\end{abox}


\begin{abox}
	Y(z) \overset{!}{=} \frac{A_1(\lambda_2) ...(z-\lambda_N) + ...+ A_N(z-\lambda_1) ... (z-\lambda_{N-1})}{HN}
\end{abox}

\begin{abox}
	Y(z) = \frac{1}{(z-(1+P))\cdot (z-1)} = \frac{A(z-1) + B(z-(1+P)) }{HN}\\ = \frac{(A+B) \cdot z - A - B(a+P)}{HN}
\end{abox}

\begin{abox}
	&-A &-(a+p)B &= 1 &(1)\\
	&A  &+B	&= 0 &(2)
\end{abox}

\begin{abox}
	(-1-p+1) \cdot B = 1 \text{ bzw. } B=-\frac{1}{p}
\end{abox}

\begin{abox}
	A= -B = \frac1p
\end{abox}

\begin{abox}
	Y(z) &= \frac{p^{-1}}{z-(a+p)} - \frac{p^{-1}}{z-1}\\
	&\ztransrueck\\
	y[k]&= p^{-1} \cdot ((1+p)^{k-1}-1)\cdot \epsilon[k-1]
\end{abox}

\begin{abox}
	Y(z) &= \frac{A}{z-5} + \frac{B}{z-3} + \frac{C}{(z-3)^2} = \frac{A(z-3)^2 + B(z-5)(z-3) C(z-5)}{HN} \\
	&= \frac{A(z^2 - 6z + 9)+ B(z^2 - 8z + 15) + C(z-5)}{HN}\\
	&= \frac{z^2(A+B)+ z(-6A-8B+C) + 9A+15B-5C}{HN}
\end{abox}

\begin{abox}
	&A + &B    &     &=2 &(1)\\
	&-6A &-8B  & +1C &=-9 &(2)\\
	&9A	 &+15B &-5C  &=3 &(3)\\
	5\cdot(2)+(3):&-21A &-25B & &=-42 &(4)\\
	21\cdot(1+4): & &-4B & &=0 &(5)
\end{abox}

\begin{abox}
	Y(z) &= \frac{2}{z-5} + \frac{3}{(z-3)^2}\\
	&\ztransrueck\\
	y[k]&= 2\cdot 5^{k-1}\epsilon[k-1] + (k-1)3^{k-1}\epsilon[k-1]
\end{abox}

\begin{abox}
	Y(z) = s(z) + \frac{r(z)}{q(z)}
\end{abox}

\begin{abox}
	s(z) &= s_0 + s_1z + ... + s_{M-N}Z^{M-N}\\
	&\ztransrueck\\
	s[k] &= s_0\delta[k] + s_1\delta[k+1] + ... + s_{M-N}\delta[k + M-N]
\end{abox}

\begin{abox}
	Y(z) &= 3z^2 - 2z + 1 \frac{2z^2 - 9z +3}{(z-5)(z-3)^2}
\end{abox}

\begin{abox}
	Y(z) &= 3z^2 - 2z + 1 \frac{2z^2 - 9z +3}{(z-5)(z-3)^2}\\
	&\ztransrueck\\
	y[k] &= 3\delta[k+2] - 2\delta[k+1] + \delta[k] + 2\cdot 5^{k-1}\epsilon[k-1] + (k-1)3^{k-1}\epsilon[k-1]
\end{abox}


\begin{abox}
	Y(z) &= \sum_{i=0}^{M-N}s_iz^i + \sum_{i=1}^{Q}\sum_{v=1}^{n_i}\frac{A_{i,v}}{(z-\lambda_i)^v}\\
	&\ztransrueck\\
	y[k]&=\sum_{i=0}^{M-N}s_i\delta[k+i] + \sum_{i=1}^{Q}\sum_{v=1}^{n_i} A_{i,v}\cdot \begin{pmatrix}
		k-1 \\v-1
	\end{pmatrix} \lambda_i^{k-v}\epsilon[k-1]
\end{abox}

\setcounter{BoxCounter}{145}
%146
\begin{abox}
	A= \frac{1}{0!}\left(\frac{d}{dz}\right)^0[(z-1) \cdot \frac{z}{z-1}(z+1)]|_{z=1}=\frac{z}{z+1}|_{z=1} = \frac12\\
	B= \frac{1}{0!}\left(\frac{d}{dz}\right)^0[(z+1) \cdot \frac{z}{z-1}(z+1)]|_{z=-1}=\frac{z}{z-1}|_{z=-1} = \frac12
\end{abox}

\begin{abox}
	\frac{A}{z \cdot \alpha} + \frac{B}{z \cdot \beta} &= \frac{\frac{a \cdot \alpha + b}{\alpha - \beta}(z - \beta) + \frac{a \cdot \beta + b}{\beta - \alpha}(z - \alpha)}{(z - a)(z - \beta)}\\
	&= \frac{z \cdot (a \cdot \alpha + b)-(a \cdot \beta + b)) - \beta(a \cdot \alpha + b) + \alpha(a \cdot \beta + b)}{(\alpha - \beta)(z - \alpha)(z - \beta)}\\
	&= \frac{z \cdot a \cdot (\alpha - \beta) + b \cdot (\alpha - \beta)}{(\alpha - \beta)(z - \alpha)(z - \beta)} = \frac{a \cdot z + b}{(z - \alpha)(z - \beta)}
\end{abox}

\begin{abox}
	A &= \frac{a \cdot \alpha + b}{\alpha - \beta} = \frac{1 \cdot 1 + 0}{1 - (-1)} = \frac{1}{2}
	B &= \frac{a \cdot \beta + b}{\alpha - \beta} = \frac{1 \cdot (-1) + 0}{-1 - 1)} = \frac{1}{2}
\end{abox}

\begin{abox}
	Y(z) = \frac{A}{z - \alpha} + \frac{B}{z - \beta} = \frac{0.5}{z - 1} + \frac{0.5}{z + 1}
\end{abox}

\begin{abox}
	\left|\lambda_i\right| < 1 \quad \forall i = 1, \dots , N
\end{abox}

\begin{abox}
	y[k] &= y[k - 1] + y[k - 2] + x[k]\\
	&\ztrans\\
	Y(z) &= z^{-1} Y(z) + z^{-2} Y(z) + X(z) \Leftrightarrow Y(z) \cdot (1 - z^{-1} - z^{-2}) = X(z)
\end{abox}

\begin{abox}
	H(z) = \frac{Y(z)}{X(z)} = \frac{1}{ (1 - z^{-1} - z^{-2})} = \frac{z^2}{z^2 - z - 1}
\end{abox}

\begin{abox}
	\lambda_{1 / 2} = \frac{-1 \pm \sqrt{1^2 + 4}}{2 \cdot 1} = \frac{1 \pm \sqrt{5}}{2}
\end{abox}

\begin{abox}
	Y(z) = H(z) \cdot X(z) = \frac{z^2}{z^2 - z - 1} \cdot z^{-1} = \frac{z}{z^2 - z - 1} = \frac{z}{(z - \lambda_1)(z - \lambda_2)}
\end{abox}

\begin{abox}
	Y(z) = \frac{1z + 0}{(z - \lambda_1)(z - \lambda_2)} = \frac{A}{z - \lambda_1} + \frac{B}{z - \lambda_2}
\end{abox}

\begin{abox}
	A &= \frac{a \cdot \alpha + b}{\alpha - \beta} = \frac{\lambda_1}{\lambda_1 - \lambda_2} = \frac{1 + \sqrt{5}}{2\sqrt{5}}\\
	B &= \frac{a \cdot \beta + b}{\alpha - \beta} = \frac{\lambda_2}{\lambda_2 - \lambda_1} = \frac{1 - \sqrt{5}}{-2\sqrt{5}}
\end{abox}

\begin{abox}
	Y(z) &= \frac{A}{z - \lambda_1} + \frac{B}{z - \lambda_2}\\
	&\ztransrueck\\
	y[k] &= A \cdot \lambda_1^{k-1} \epsilon[k - 1] +  B \cdot \lambda_2^{k-1} \epsilon[k - 1]\\
	&= \frac{1 + \sqrt{5}}{2\sqrt{5}} \cdot \left(\frac{1 + \sqrt{5}}{2}\right)^{k -1} \cdot \epsilon[k - 1] +  \frac{1 - \sqrt{5}}{-2\sqrt{5}} - \frac{1 - \sqrt{5}}{-2\sqrt{5}} \cdot \left(\frac{1 + \sqrt{5}}{2}\right)^{k - 1} \cdot \epsilon[k - 1]\\
	&= \frac{1}{\sqrt{5}}\left(\left(\frac{1 + \sqrt{5}}{2}\right)^k - \left(\frac{1 - \sqrt{5}}{2}\right)^k\right)\epsilon[k - 1]
\end{abox}

\begin{abox}
	U(z) &= H_1(z) \cdot X(z) \text{ und}\\
	Y(z) &= H_2(z) \cdot U(z) = H_2(z) \cdot H_1(z) \cdot X(z)
\end{abox}

\begin{abox}
	H(z) &= \frac{Y(z)}{X(z)} = H_1(z) \cdot H_2(z)\\
	&\ztransrueck\\
	h[k] &= h_1[k] \ast h_2[k]
\end{abox}

\begin{abox}
	V(z) &= H_1(z) \cdot X(z) \text{ und}\\
	W(z) &= H_2(z) \cdot X(z) \text{ und also } Y(z) = V(z) + W(z) = H_1(z) \cdot X(z) + H_2(z) \cdot X(z) = (H_1(z) + H_2(z)) \cdot X(z)
\end{abox}

\begin{abox}
	H(z) &:= \frac{Y(z)}{X(z)} = H_1(z) + H_2(z)\\
	&\ztransrueck\\
	h[k] &= h_1[k] + h_2[k]
\end{abox}

\begin{abox}
	V(z) &= X(z) - W(z) \text{ und } W(z) = H_2(z) \cdot Y(z) \text{ und}\\
	Y(z) &= V(z) \cdot H_1(z) = H_1(z) \cdot (X(z) \cdot H_2(z) \cdot Y(z))\\
	&= H_1(z) \cdot X(z) - H_1(z) \cdot H_2(z) \cdot Y(z)\\
	&\Leftrightarrow Y(z) \cdot (1 + H_1(z) + H_2(z)) = H_1(z) \cdot X(z)
\end{abox}

\begin{abox}
	H(z) = \frac{Y(z)}{X(z)} = \frac{H_1(z)}{1 + H_1(z) + H_2(z)}
\end{abox}

\begin{abox}
	H(z) = H_1(z) \cdot H_2(z) = \frac{(z + 3)(z - 1)}{(z^2 - 1)(z + 3)(z - 1)} = \frac{1}{(z - 1)^2} = \frac{1}{z^2 - 2z - 1}
\end{abox}

\begin{abox}
	y[k] - 2y[k - 1] + y[k - 2] = x[k - 2]
\end{abox}

\begin{abox}
	y[k] = 2y[k] - y[k - 2] + x[k - 2]
\end{abox}

\begin{abox}
	H(z) &= H_1(z) + H_2(z) = \frac{z + 3}{z^2 - 1} + \frac{z + 1}{(z + 3)(z - 1)} = \frac{(z + 3)^2 + (z + 1)^2}{(z^2 - 1)(z + 3)}\\
	&= \frac{2z^2 + 8z + 10}{z^3 + 3z^2 - z - 3} \text{ (Systemfunktion)}\\
	y[k] &+ 3y[k - 1] - y[k - 2] - 3y[k - 3] = 2x[k - 1] + 8x[k - 2] + 10x[k - 3] \text{ (DLG)}\\
	y[k] &= 2x[k - 1] + 8x[k - 2] + 10x[k - 3] - 3y[k - 1] + y[k - 2] + 3y[k - 3] \text{ (Alg.)}
\end{abox}

\begin{abox}
	H(z) &= \frac{H_1(z)}{1 + H_1(z) + H_2(z)} = \frac{\frac{z + 3}{z^2 - 1}}{1 + \frac{(z + 3)(z + 1)}{(z^2 - 1)(z + 3)(z - 1)}} = \frac{\frac{z + 3}{z^2 - 1}}{\frac{(z - 1)^2 + 1}{(z - 1)^2}} = \frac{\frac{z + 3}{z + 1}}{\frac{z^2 - 2z + 2}{z - 1}}\\
	&= \frac{(z + 3)(z - 1)}{(z + 1)(z^2 - 2z + 2)} = \frac{z^2 + 2z - 3}{z^3 - z^2 + 2} \text{ (Systemfunktion)}\\
	y[k] &- y[k - 1] + 2y[k - 3] = x[k - 1] + 2x[k - 2] + 3x[k - 3] \text{ (DLG)}\\
	y[k] &= x[k - 1] + 2x[k - 2] - 3x[k - 3] + y[k - 1] - 2y[k - 3] \text{ (Alg.)}
\end{abox}

\begin{abox}
	\int_{a}^{b}f(t)dt := \lim\limits_{n \to \infty}\sum_{i = 0}^{n - 1}f(a + i \cdot \varDelta t_n)
\end{abox}

\begin{abox}
	\varDelta t_n = \frac{b - a}{n}
\end{abox}


\chapter{Kontinuierliche Signale}

\begin{abox}
	Inhalt...
\end{abox}

\setcounter{BoxCounter}{170}

\begin{abox}
	\int_{-\infty}^{t} \epsilon(\tau)d\tau= \begin{cases}
		0 &, t\leq 0\\
		\int_{0}^{1}1d\tau=[\tau]_0^t = t &,t>0
	\end{cases} \quad = t\cdot \epsilon(t) =: ramp(t)
\end{abox}

\begin{abox}
	\int_{-\infty}^{t}\delta(\tau)d\tau = \epsilon(t)
\end{abox}

\begin{abox}
	\delta(t):= \frac{d}{dt}\epsilon(t) &= \lim\limits_{T \to 0} \frac1T \text{rect}(\frac{t}{T})
	&= \lim\limits_{T \to 0} \frac{1}{T} \text{tri}(\frac{t}{T}) = 
	\lim\limits_{T \to 0} \frac2T \text{si}(s\pi\frac{t}{T})
\end{abox}

\begin{tbox}
	\begin{enumerate}[label=\Roman*)]
		\item $x(\tau) \cdot \delta(\tau - t) = x(t) \cdot \delta(\tau - t)$
		\item $\int_{-\infty}^{\infty}\delta(\tau - t)d\tau = 1$
		\item $x(t) = \int_{-\infty}^{\infty}x(\tau)\delta(t-\tau)d\tau$ fÃ¼r alle $ t \in \mathbb{R}$
	\end{enumerate}
\end{tbox}

\begin{abox}
	\int_{-\infty}^{\infty}\delta(\tau - t)d\tau = \int_{-\infty}^{\infty}\delta(\lambda)d\lambda = \epsilon(\infty) = 1
\end{abox}


\begin{abox}
	\int_{-\infty}^{\infty}x(\tau)\delta(t  - \tau) d \tau &= 	\int_{-\infty}^{\infty}x(\tau)\delta(\tau - t) d \tau \overset{(I)}{=}	\int_{-\infty}^{\infty}x(t)\delta(\tau -t) d \tau \\
	&= x(t)	\int_{-\infty}^{\infty}\delta(\tau - t) d \tau \overset{(II)}{=} x(t) \cdot 1 = x(t)
\end{abox}

\begin{abox}
	(x * y) (t) := 	\int_{-\infty}^{\infty}x(\tau)y(t  - \tau) d \tau
\end{abox}

\begin{tbox}
	a) \begin{align*}\epsilon(t) * \epsilon(t) = \int_{-\infty}^{\infty}\epsilon(\tau)\epsilon(t  - \tau) d \tau = 
	\int_{0}^{\infty}\epsilon(t  - \tau) d \tau = 	\int_{0}^{t}1 \cdot d\tau \overset{\lambda := t-\tau}{=}\\
	-\int_{t}^{-\infty}\epsilon(\lambda) d \lambda = 
	\int_{-\infty}^{0}\epsilon(\lambda) d \lambda \overset{(42)}{=} t\epsilon(t) = \text{ramp}(t)\end{align*}
	b) \begin{align*}
	\text{rect}(t) * \epsilon(t) &= 	\int_{-\infty}^{\infty}\rect(\tau)\epsilon(t  - \tau) d \tau \\&= 
	\int_{-0,5}^{0,5}\epsilon(t  - \tau) d \tau \overset{\lambda := t-\tau}{=}
	-\int_{t-(-0,5)}^{t-0,5}\epsilon(\lambda) d \lambda = 
	-\int_{t-0,5)}^{t+0,5}\epsilon(\lambda) d \lambda\\ &\overset{(4.2)}{=}[\lambda\epsilon(\lambda)]_{t-0,5}^{t+0,5}
	= \ramp(t+0,5) - \ramp(t-0,5)\\
	&= \begin{cases}
	0 &, t \leq -0,5\\
	t+0,5 &, -0,5 \leq t \leq 0,5\\
	1 &, t \geq 0,5
	\end{cases} =: \sramp
	\end{align*}
\end{tbox}

\begin{tbox}
	c) \begin{align*}
	\rect(t) * \epsilon(t) &= (\epsilon(t+0,5) - \epsilon(t-0,5)) * \epsilon(t)\\
	&\overset{(III)}{=}\epsilon(t +0,5) * \epsilon(t) - \epsilon(t-0,5) * \epsilon(t)\\
	&\overset{(VI.a)}{=} \ramp(t + 0,5) - \ramp( t - 0,5) = sramp(t)
	\end{align*}
\end{tbox}

\begin{abox}
	\cos\Phi = \frac{\left\langle x(t), y(t)\right\rangle}{\left\|x(t)|\right\| \cdot \left\|y(t)\right\|}
\end{abox}

\begin{abox}
	E_{\delta(t-\tau)} = \left\|\delta(t-\tau)\right\|^2 = \int_{-\infty}^{\infty} \delta^2(t-\tau)dt = \lim\limits_{T \to \infty} \int_{\tau -\frac{T}{2}}^{\tau +\frac{T}{2}}\frac{a}{T^2}dt = \lim\limits_{T \to \infty} \frac{a}{T} = \infty\\
	\cos\Phi = \frac{\left\langle \delta(t-\tau_1), \delta(t-\tau_2)\right\rangle}{\left\|\delta(t-\tau_1)|\right\| \cdot \left\|\delta(t-\tau_2)\right\|} = \frac{\int_{-\infty}^{\infty}\delta(t-\tau_1)\cdot \delta(t-\tau_2)dt}{\infty \cdot \infty} = \frac{\int_{-\infty}^{\infty}0dt}{\infty}=0
\end{abox}

\begin{abox}
	\|\rect(t-\tau)\|^2 &= \int_{-\infty}^{\infty}\rect^2(t-\tau)dt \overset{\lambda = t-\tau}{=} \int_{-\infty}^{\infty}\rect(\lambda)d\lambda\overset{(Def.rect)}{=} 1\\
	\cos\Phi &= \frac{\langle \rect(t-\tau_1), \rect(t-\tau_2)\rangle}{\|\rect(t-\tau_1)\| \cdot \|\rect(t-\tau_2)\|} \\
	&=
	\frac{\int_{-\infty}^{\infty}\rect(\lambda)\cdot \rect(\lambda-((\tau_2 - \tau_1)))d\lambda}{1 \cdot 1}\\
	&\overset{(symm rect)}{=} int_{-\infty}^{\infty}\rect(\lambda)\rect((\tau_2 - \tau_1) - \lambda) d\lambda\\
	&\overset{(Def. Faltung)}{=} (\rect * \rect)(\tau_2 - \tau_1)\\
	&\overset{S91, Bsp. d}{=} \tri(\tau_2 -  \tau_1)\\
	\implies \Phi &= \arccos \tri(\tau_2 - \tau_1)
\end{abox}

\begin{abox}
	\langle &\sin(n\omega_0t),\sin(m\omega_0t)\rangle_T = \int_{-\frac{T}{2}}^{\frac{T}{2}}\frac{1}{2j}(e^{jn\omega_0t}-e^{-jn\omega_0t}) \cdot \frac{1}{2j}(e^{jm\omega_0t}-e^{-jm\omega_0t}) dt\\
	&=-\frac{1}{4}\int_{-\frac{T}{2}}^{\frac{T}{2}}e^{j(n+m)\omega_0t}-e^{j(m-n)\omega_0t}-e^{j(n.m)\omega_0t}+e^{-j(n+m)\omega_0t}dt\\
	&\overset{(4.12)}{=}-\frac{T}{4}(\delta[n+m] - \delta[m-n] - \delta[n-m] - \delta[-(n+m)])\\
	&= \frac{T}{4}\cdot(2\delta[n-m] - 2\delta[n+m]) = \frac{T}{2}\delta[n-m] = \begin{cases}
		0 &,n\ne m\\
		\frac{T}{2}&, n = m \ne 0
	\end{cases}
\end{abox}

\todo{insert Boxes 184 -196}

\setcounter{BoxCounter}{196}
\begin{abox}
	x_F(t) \approx \frac{0.5}{2} &+ 0.45\cos(\omega_0 t) + 0.15\cos(3\omega_0 t)\\
	&+ 0 \cdot \cos(4\omega_0 t) - 0.09  \cos(5\omega_0 t)
\end{abox}

\begin{abox}
	r_n\cos(\underbrace{n\omega_0t}_{\alpha} - \underbrace{\varphi_n}_{\beta}) &= \underbrace{r_n \cdot \cos(\varphi_n)}_{:= a_n} \cdot \cos(n\omega_0t)+ \underbrace{r_n \cdot \sin(\varphi_n)}_{:= b_n} \cdot \sin(n\omega_0t)\\
	&= a_n\cos(n\omega_0t) + b_n \sin(n\omega_0t)
\end{abox}

\begin{dbox}[width=0.7\textwidth]
	\begin{align*}
	r_n &= \sqrt{a_n^2 + b_n^2} \text{ und } \varphi_n = \overset{~}{sgn}(b_n)\cdot\arccos\frac{a_n}{r_n}\\
	&(\text{bzw. } \varphi_n = \arctan\left(\frac{b_n}{a_n}\right) + \pi \cdot (1 - \epsilon(a_n)\cdot\overset{~}{sgn}(b_n)))
	\end{align*}
\end{dbox}

\begin{abox}
	r_0 &= \frac{a_0}{2} = \hat{x} \frac{T_i}{T}\\
	r_n &= \sqrt{a_n^2 + b_n^2} = \left|a_n\right| = 2\hat{x}\frac{T_i}{T} \cdot \left|si\left(n\pi\frac{T_i}{T}\right)\right|
\end{abox}


